@prefix  sh:   <http://raw.github.com/jneubert/skos-history/master/skos-history.ttl/> .
@prefix  dc:   <http://purl.org/dc/elements/1.1/> .
@prefix  dcterms: <http://purl.org/dc/terms/> .
@prefix  dsv:  <http://purl.org/iso25964/DataSet/Versioning#> .
@prefix  owl:  <http://www.w3.org/2002/07/owl#> .
@prefix  rdf:  <http://www.w3.org/1999/02/22-rdf-syntax-ns#> .
@prefix  rdfs: <http://www.w3.org/2000/01/rdf-schema#> .
@prefix  sd:   <http://www.w3.org/ns/sparql-service-description#> .
@prefix  skos: <http://www.w3.org/2004/02/skos/core#> .
@prefix  xsd:  <http://www.w3.org/2001/XMLSchema#> .

# Ontology

<http://raw.github.com/jneubert/skos-history/master/skos-history.ttl/>
    a owl:Ontology ;
    dc:creator "Joachim Neubert" ;
    dc:title "skos-history - Ontology for expressing version deltas of SKOS files"@en ;
    dcterms:created "2013-09-02"^^xsd:date ;
    dcterms:modified "2014-10-24"^^xsd:date ;
    dc:date "2014-10-24" ;
    rdfs:comment """This ontology proposal is meant to support comparisons between versions of SKOS vocabularies, both on the level of single concepts and on the level of aggregations of certain types of changes. The version deltas are expressed as graphs of insertions and deletions.
The ontology may be used in conjunction with the proposed dataset versioning ontology (http://purl.org/iso25964/DataSet/Versioning#) for addressing the versions of a (SKOS) dataset via their related version history records."""@en .

# Classes

sh:SchemeDelta
    a rdfs:Class ;
    rdfs:isDefinedBy <http://raw.github.com/jneubert/skos-history/master/skos-history.ttl> ;
    rdfs:label "Scheme Delta"@en ;
    rdfs:subClassOf skos:ConceptScheme ;
    rdfs:comment "The delta of two versions of a SKOS concept scheme."@en .

sh:SchemeDeltaInsertions
    a rdfs:Class ;
    rdfs:comment """Should be related to the delta by dcterms:isPartOf."""@en ;
    rdfs:isDefinedBy <http://raw.github.com/jneubert/skos-history/master/skos-history.ttl> ;
    rdfs:label "Scheme Delta Insertions"@en ;
    rdfs:subClassOf skos:ConceptScheme ;
    rdfs:comment "The statements to insert into one version of a SKOS concept scheme to create another version (in addition to deletions)."@en .

sh:SchemeDeltaDeletions
    a rdfs:Class ;
    rdfs:comment """Should be related to the delta by dcterms:isPartOf."""@en ;
    rdfs:isDefinedBy <http://raw.github.com/jneubert/skos-history/master/skos-history.ttl> ;
    rdfs:label "Scheme Delta Deletions"@en ;
    rdfs:subClassOf skos:ConceptScheme ;
    rdfs:comment "The statements to delete from one version of a SKOS concept scheme to create another version (in addition to insertions)."@en .

# TODO are these needed??

sh:ConceptVersion
    a rdfs:Class ;
    rdfs:comment """Should be related to the concept by dcterms:isVersionOf."""@en ;
    rdfs:isDefinedBy <http://raw.github.com/jneubert/skos-history/master/skos-history.ttl> ;
    rdfs:label "Concept Version"@en ;
    rdfs:subClassOf skos:Concept ;
    rdfs:comment "(???) A version of a SKOS concept."@en .

sh:ConceptDelta
    a rdfs:Class ;
    rdfs:isDefinedBy <http://raw.github.com/jneubert/skos-history/master/skos-history.ttl> ;
    rdfs:label "Concept Delta"@en ;
    # TODO that's not true!
    # rdfs:subClassOf skos:Concept ;
    rdfs:comment "The delta of two versions of a SKOS concept."@en .

# Properties

sh:usingNamedGraph
    a owl:ObjectProperty ;
    rdfs:isDefinedBy <http://raw.github.com/jneubert/skos-history/master/skos-history.ttl> ;
    rdfs:label "using Named Graph"@en ;
    # TODO
    #rdfs:subPropertyOf <???> ;
    rdfs:range sd:NamedGraph ;
    rdfs:comment "The named graph where the data can be queried. (The endpoint should be given as void:sparqlEndpoint property of the version history set.)"@en .

sh:deltaFrom
    a owl:ObjectProperty ;
    rdfs:isDefinedBy <http://raw.github.com/jneubert/skos-history/master/skos-history.ttl> ;
    rdfs:label "delta From"@en ;
    # TODO
    #rdfs:subPropertyOf <???> ;
    rdfs:domain sh:SchemeDelta ;
    rdfs:comment "The version from which the delta is taken. The object of the triple may be a dsv:VersionHistoryRecord."@en .

sh:deltaTo
    a owl:ObjectProperty ;
    rdfs:isDefinedBy <http://raw.github.com/jneubert/skos-history/master/skos-history.ttl> ;
    rdfs:label "delta To"@en ;
    # TODO
    #rdfs:subPropertyOf <???> ;
    rdfs:domain sh:SchemeDelta ;
    rdfs:comment "The versions to which the delta is taken. The object of the triple may be a dsv:VersionHistoryRecord."@en .

sh:hasDelta
    a owl:ObjectProperty ;
    rdfs:isDefinedBy <http://raw.github.com/jneubert/skos-history/master/skos-history.ttl> ;
    rdfs:label "has Delta"@en ;
    # TODO
    #rdfs:subPropertyOf <???> ;
    rdfs:range sh:SchemeDelta ;
    rdfs:comment "A delta for this version. The subject of the triple may be a dsv:VersionHistoryRecord."@en .

# TODO check the following properties as possibly obsolete when using delta ontology

sh:concepthistory
    a owl:ObjectProperty ;
    rdfs:isDefinedBy <http://raw.github.com/jneubert/skos-history/master/skos-history.ttl> ;
    rdfs:label "concept History"@en ;
    # TODO
    #rdfs:subPropertyOf <???> ;
    rdfs:Comment "Collects the concept deltas of a concept (given in the subject of the triple)."@en .

sh:prefLabelInsertion
    a owl:ObjectProperty ;
    rdfs:isDefinedBy <http://raw.github.com/jneubert/skos-history/master/skos-history.ttl> ;
    rdfs:label "prefLabel Insertion"@en ;
    # TODO
    #rdfs:subPropertyOf <???> ;
    rdfs:comment "skos:prefLabel which is to be inserted."@en .

sh:prefLabelDeletion
    a owl:ObjectProperty ;
    rdfs:isDefinedBy <http://raw.github.com/jneubert/skos-history/master/skos-history.ttl> ;
    rdfs:label "prefLabel Deletion"@en ;
    # TODO
    #rdfs:subPropertyOf <???> ;
    rdfs:comment "skos:prefLabel which is to be deleted."@en .

